\documentclass{article}
\usepackage{tikz}
\begin{document}

\begin{tikzpicture}
  \node[right of=a, label={[label distance=2]above right:b}] {};
  \node (c) [below of=a, label={[label distance=4]below left:c}] {};
  \node (c) [below of=a, label={[label distance=4]below left:c}] {};
  \node (c) [below of=a, label={[label distance=4]below left:c}] {};
  \node (c) [below of=a, label={[label distance=4]below left:c}] {};
  \node (c) [below of=a, label={[label distance=4]below left:c}] {};
  \node (c) [below of=a, label={[label distance=4]below left:c}] {};
  \node (c) [below of=a, label={[label distance=4]below left:c}] {};
\end{tikzpicture}

  \begin{equation}
    \label{eq:1}
    1 + 1 = 2
  \end{equation}
\end{document}